CPolyEquiv/CPolyEquiv.lean
@@ -1,3 +1,4 @@
 import CPolyEquiv.Generated
 import CPolyEquiv.Equiv
 import CPolyEquiv.EquivMl
+import CPolyEquiv.Check
